FAIL: make nondep_then, etc. abstract

src/lowparse/LowParse.Spec.Combinators.fst
@@ -232,6 +232,23 @@ let and_then_cases_injective
   and_then_cases_injective_precond p' x1 x2 b1 b2 ==>
   x1 == x2
 
+let and_then_cases_injective_intro
+  (#t:Type)
+  (#t':Type)
+  (p': (t -> Tot (bare_parser t')))
+  (lem: (
+    (x1: t) -> 
+    (x2: t) ->
+    (b1: bytes) ->
+    (b2: bytes) ->
+    Lemma
+    (requires (and_then_cases_injective_precond p' x1 x2 b1 b2))
+    (ensures (x1 == x2))
+  ))
+: Lemma
+  (and_then_cases_injective p')
+= Classical.forall_intro_3 (fun x1 x2 b1 -> Classical.forall_intro (Classical.move_requires (lem x1 x2 b1)))
+
 val and_then_injective
   (#t:Type)
   (#t':Type)
@@ -412,6 +429,7 @@ let and_then_correct
 
 #reset-options
 
+abstract
 val and_then
   (#k: parser_kind)
   (#t:Type)
@@ -430,8 +448,23 @@ let and_then #k #t p #k' #t' p' =
   and_then_correct p p' ;
   f
 
+abstract
+let and_then_eq
+  (#k: parser_kind)
+  (#t:Type)
+  (p:parser k t)
+  (#k': parser_kind)
+  (#t':Type)
+  (p': (t -> Tot (parser k' t')))
+  (input: bytes)
+: Lemma
+  (requires (and_then_cases_injective p'))
+  (ensures (parse (and_then p p') input == and_then_bare p p' input))
+= ()
+
 (* Special case for non-dependent parsing *)
 
+abstract
 let nondep_then
   (#k1: parser_kind)
   (#t1: Type0)
@@ -444,6 +477,7 @@ let nondep_then
 
 #set-options "--z3rlimit 16"
 
+abstract
 let nondep_then_eq
   (#k1: parser_kind)
   (#t1: Type0)
@@ -537,6 +571,7 @@ let bare_serialize_nondep_then_correct
   in
   Classical.forall_intro prf
 
+abstract
 let serialize_nondep_then
   (#k1: parser_kind)
   (#t1: Type0)
@@ -551,6 +586,23 @@ let serialize_nondep_then
 = bare_serialize_nondep_then_correct p1 s1 p2 s2;
   bare_serialize_nondep_then p1 s1 p2 s2
 
+abstract
+let serialize_nondep_then_eq
+  (#k1: parser_kind)
+  (#t1: Type0)
+  (p1: parser k1 t1)
+  (s1: serializer p1)
+  (u: unit { k1.parser_kind_subkind == Some ParserStrong } )
+  (#k2: parser_kind)
+  (#t2: Type0)
+  (p2: parser k2 t2)
+  (s2: serializer p2)
+  (input: t1 * t2)
+: Lemma
+  (serialize (serialize_nondep_then p1 s1 u p2 s2) input == bare_serialize_nondep_then p1 s1 p2 s2 input)
+= ()
+
+abstract
 let serialize_nondep_then_upd_left
   (#k1: parser_kind)
   (#t1: Type0)
@@ -576,6 +628,7 @@ let serialize_nondep_then_upd_left
   Seq.lemma_split s l1;
   Seq.lemma_append_inj (Seq.slice s 0 l1) (Seq.slice s l1 (Seq.length s)) (serialize s1 (fst x)) (serialize s2 (snd x))
 
+abstract
 let serialize_nondep_then_upd_left_chain
   (#k1: parser_kind)
   (#t1: Type0)
@@ -610,6 +663,7 @@ let serialize_nondep_then_upd_left_chain
   seq_upd_seq_right_to_left s 0 s1' i' s';
   seq_upd_seq_slice_idem s 0 (Seq.length s1')
 
+abstract
 let serialize_nondep_then_upd_bw_left
   (#k1: parser_kind)
   (#t1: Type0)
@@ -634,6 +688,7 @@ let serialize_nondep_then_upd_bw_left
 
 #reset-options "--z3refresh --z3rlimit 64 --z3cliopt smt.arith.nl=false"
 
+abstract
 let serialize_nondep_then_upd_bw_left_chain
   (#k1: parser_kind)
   (#t1: Type0)
@@ -664,6 +719,7 @@ let serialize_nondep_then_upd_bw_left_chain
   serialize_nondep_then_upd_left_chain p1 s1 u p2 s2 x y j' s';
   assert (j' == Seq.length (serialize (serialize_nondep_then p1 s1 u p2 s2) x) - (Seq.length (serialize s2 (snd x)) + i') - Seq.length s')
 
+abstract
 let serialize_nondep_then_upd_right
   (#k1: parser_kind)
   (#t1: Type0)
@@ -689,6 +745,7 @@ let serialize_nondep_then_upd_right
   Seq.lemma_split s l2;
   Seq.lemma_append_inj (Seq.slice s 0 l2) (Seq.slice s l2 (Seq.length s)) (serialize s1 (fst x)) (serialize s2 (snd x))
 
+abstract
 let serialize_nondep_then_upd_right_chain
   (#k1: parser_kind)
   (#t1: Type0)
@@ -725,6 +782,7 @@ let serialize_nondep_then_upd_right_chain
   seq_upd_seq_right_to_left s l2 s2' i' s';
   seq_upd_seq_slice_idem s l2 (Seq.length s)
 
+abstract
 let serialize_nondep_then_upd_bw_right
   (#k1: parser_kind)
   (#t1: Type0)
@@ -746,6 +804,7 @@ let serialize_nondep_then_upd_bw_right
   ))
 = serialize_nondep_then_upd_right p1 s1 u p2 s2 x y
 
+abstract
 let serialize_nondep_then_upd_bw_right_chain
   (#k1: parser_kind)
   (#t1: Type0)
@@ -920,6 +979,18 @@ let synth_injective_intro
   (ensures (synth_injective f))
 = ()
 
+let parse_synth'
+  (#k: parser_kind)
+  (#t1: Type0)
+  (#t2: Type0)
+  (p1: parser k t1)
+  (f2: t1 -> GTot t2)
+: Tot (bare_parser t2)
+= fun b -> match parse p1 b with
+  | None -> None
+  | Some (x1, consumed) -> Some (f2 x1, consumed)
+
+abstract
 let parse_synth
   (#k: parser_kind)
   (#t1: Type0)
@@ -933,6 +1004,7 @@ let parse_synth
   (ensures (fun _ -> True))
 = coerce (parser k t2) (and_then p1 (fun v1 -> parse_fret f2 v1))
 
+abstract
 let parse_synth_eq
   (#k: parser_kind)
   (#t1: Type0)
@@ -942,9 +1014,7 @@ let parse_synth_eq
   (b: bytes)
 : Lemma
   (requires (synth_injective f2))
-  (ensures (parse (parse_synth p1 f2) b == (match parse p1 b with
-  | None -> None
-  | Some (x1, consumed) -> Some (f2 x1, consumed))))
+  (ensures (parse (parse_synth p1 f2) b == parse_synth' p1 f2 b))
 = ()
 
 let compose (#t1 #t2 #t3: Type) (f1: t1 -> GTot t2) (f2: t2 -> GTot t3) (x: t1) : GTot t3 =
@@ -1037,6 +1107,7 @@ let synth_inverse_synth_injective'
 : Tot (squash (synth_injective f))
 = ()
 
+abstract
 let serialize_synth
   (#k: parser_kind)
   (#t1: Type0)
@@ -1053,6 +1124,7 @@ let serialize_synth
 = bare_serialize_synth_correct p1 f2 s1 g1;
   bare_serialize_synth p1 f2 s1 g1
 
+abstract
 let serialize_synth_eq
   (#k: parser_kind)
   (#t1: Type0)
@@ -1070,6 +1142,7 @@ let serialize_synth_eq
   (serialize (serialize_synth p1 f2 s1 g1 u) x == serialize s1 (g1 x))
 = ()
 
+abstract
 let serialize_synth_upd_chain
   (#k: parser_kind)
   (#t1: Type0)
@@ -1104,6 +1177,7 @@ let serialize_synth_upd_chain
   ))
 = ()
 
+abstract
 let serialize_synth_upd_bw_chain
   (#k: parser_kind)
   (#t1: Type0)
@@ -1196,6 +1270,7 @@ let parse_filter_payload
     else fail_parser parse_filter_payload_kind (x: t {f x == true} )
   )
 
+abstract
 let parse_filter
   (#k: parser_kind)
   (#t: Type0)
@@ -1204,6 +1279,7 @@ let parse_filter
 : Tot (parser (parse_filter_kind k) (x: t { f x == true }))
 = p `and_then` (parse_filter_payload f)
 
+abstract
 let parse_filter_eq
   (#k: parser_kind)
   (#t: Type0)
